Tidy up envLang obs. sem. definition (more work needed)

compiler/backend/env_semanticsScript.sml
@@ -6,41 +6,40 @@ open stringTheory optionTheory sumTheory pairTheory listTheory alistTheory
      pure_semanticsTheory pure_configTheory
      thunkLang_primitivesTheory envLangTheory io_treeTheory;
 
-val _ = new_theory "envLang_semantics";
+val _ = new_theory "env_semantics";
 
 val _ = set_grammar_ancestry ["envLang", "io_tree"];
 
 
 (******************** Datatypes and helpers ********************)
 
-(* TODO: we could make the equivalent types in pure_semantics parametric and re-use *)
 Datatype:
-  tcont = Done        (* nothing left to do *)
-        | BC v tcont (* RHS of Bind, rest *)
-        | HC v tcont (* RHS of Handle, rest *)
+  cont = Done      (* nothing left to do *)
+       | BC v cont (* RHS of Bind, rest *)
+       | HC v cont (* RHS of Handle, rest *)
 End
 
-Type tstate[pp] = “:(v list) list”;
+Type state[pp] = “:(v list) list”;
 
 Datatype:
-  tnext_res = Act 'e tcont tstate | Ret | Div | Err
+  next_res = Act 'e cont state | Ret | Div | Err
 End
 
-Definition tget_atoms_def:
-  tget_atoms [] = SOME [] ∧
-  tget_atoms (Atom a :: xs) = OPTION_MAP (λas. a::as) (tget_atoms xs) ∧
-  tget_atoms _ = NONE
+Definition get_atoms_def:
+  get_atoms [] = SOME [] ∧
+  get_atoms (Atom a :: xs) = OPTION_MAP (λas. a::as) (get_atoms xs) ∧
+  get_atoms _ = NONE
 End
 
-Definition twith_atoms_def:
-  twith_atoms vs f =
-    case tget_atoms vs of
+Definition with_atoms_def:
+  with_atoms vs f =
+    case get_atoms vs of
     | SOME as => f as
     | NONE => Err
 End
 
-Definition tapply_closure_def:
-  tapply_closure f arg cont =
+Definition apply_closure_def:
+  apply_closure f arg cont =
     case dest_anyClosure f of
     | INR (x, env, body) => cont (eval (env ++ [(x,arg)]) body)
     | _ => Err
@@ -50,7 +49,7 @@ End
 (******************** Intermediate definitions ********************)
 
 Definition next_def:
-  next (k:num) sv stack (state:tstate) =
+  next (k:num) sv stack (state:state) =
     case sv of
     | INL Diverge => Div
     | INL _ => Err
@@ -61,7 +60,7 @@ Definition next_def:
             (case stack of
              | Done => Ret
              | BC f fs =>
-                tapply_closure f (HD vs)
+                apply_closure f (HD vs)
                   (λw. if k = 0 then Div else next (k-1) w fs state)
              | HC f fs => if k = 0 then Div else next (k-1) sv fs state)
           else if s = "Raise" ∧ LENGTH vs = 1 then
@@ -69,7 +68,7 @@ Definition next_def:
              | Done => Ret
              | BC f fs => if k = 0 then Div else next (k-1) sv fs state
              | HC f fs =>
-                tapply_closure f (HD vs)
+                apply_closure f (HD vs)
                   (λw. if k = 0 then Div else next (k-1) w fs state))
           else if s = "Bind" ∧ LENGTH vs = 2 then
             (let m = EL 0 vs in
@@ -80,12 +79,12 @@ Definition next_def:
              let f = EL 1 vs in
                if k = 0 then Div else next (k-1) (INR m) (HC f stack) state)
           else if s = "Act" ∧ LENGTH vs = 1 then
-            (twith_atoms vs (λas.
+            (with_atoms vs (λas.
                case HD as of
                | Msg channel content => Act (channel, content) stack state
                | _ => Err))
           else if s = "Alloc" ∧ LENGTH vs = 2 then
-            (twith_atoms [HD vs] (λas.
+            (with_atoms [HD vs] (λas.
                case HD as of
                | Int len =>
                    (let n = if len < 0 then 0 else Num len in
@@ -96,7 +95,7 @@ Definition next_def:
                           stack new_state)
                | _ => Err))
           else if s = "Length" ∧ LENGTH vs = 1 then
-            (twith_atoms vs (λas.
+            (with_atoms vs (λas.
                case HD as of
                | Loc n =>
                    (if LENGTH state ≤ n then Err else
@@ -106,7 +105,7 @@ Definition next_def:
                         stack state)
                | _ => Err))
           else if s = "Deref" ∧ LENGTH vs = 2 then
-            (twith_atoms vs (λas.
+            (with_atoms vs (λas.
                case (EL 0 as, EL 1 as) of
                | (Loc n, Int i) =>
                    (if LENGTH state ≤ n then Err else
@@ -121,7 +120,7 @@ Definition next_def:
                         stack state)
                | _ => Err))
           else if s = "Update" ∧ LENGTH vs = 3 then
-            (twith_atoms [EL 0 vs; EL 1 vs] (λas.
+            (with_atoms [EL 0 vs; EL 1 vs] (λas.
                case (EL 0 as, EL 1 as) of
                | (Loc n, Int i) =>
                    (if LENGTH state ≤ n then Err else
@@ -203,7 +202,7 @@ End
 
 (******************** Lemmas ********************)
 
-Theorem tnext_less_eq:
+Theorem next_less_eq:
   ∀n e k st m.
     next n e k st ≠ Div ∧
     n ≤ m
@@ -219,35 +218,35 @@ Proof
   Cases_on `s = "Raise"` >> gvs[]
   >- (
     IF_CASES_TAC >> gvs[] >> TOP_CASE_TAC >> gvs[] >- (IF_CASES_TAC >> gvs[]) >>
-    simp[tapply_closure_def] >> rpt $ TOP_CASE_TAC >> gvs[]
+    simp[apply_closure_def] >> rpt $ TOP_CASE_TAC >> gvs[]
     ) >>
   Cases_on `s = "Ret"` >> gvs[]
   >- (
     IF_CASES_TAC >> gvs[] >>
     reverse $ TOP_CASE_TAC >> gvs[] >- (IF_CASES_TAC >> gvs[]) >>
-    simp[tapply_closure_def] >> rpt $ TOP_CASE_TAC >> gvs[]
+    simp[apply_closure_def] >> rpt $ TOP_CASE_TAC >> gvs[]
     ) >>
   Cases_on `s = "Alloc"` >> gvs[]
   >- (
-    IF_CASES_TAC >> gvs[] >> rw[twith_atoms_def] >>
+    IF_CASES_TAC >> gvs[] >> rw[with_atoms_def] >>
     ntac 3 (TOP_CASE_TAC >> gvs[]) >>
     first_x_assum irule >> simp[] >> qexists_tac `[Int i]` >> simp[]
     ) >>
   Cases_on `s = "Length"` >> gvs[]
   >- (
-    IF_CASES_TAC >> gvs[] >> rw[twith_atoms_def] >>
+    IF_CASES_TAC >> gvs[] >> rw[with_atoms_def] >>
     ntac 4 (TOP_CASE_TAC >> gvs[]) >>
     first_x_assum irule >> simp[] >> qexists_tac `[Loc n]` >> simp[]
     ) >>
   Cases_on `s = "Deref"` >> gvs[]
   >- (
-    IF_CASES_TAC >> gvs[] >> rw[twith_atoms_def] >>
+    IF_CASES_TAC >> gvs[] >> rw[with_atoms_def] >>
     ntac 6 (TOP_CASE_TAC >> gvs[]) >>
     first_x_assum irule >> simp[] >> qexists_tac `[Loc n; Int i]` >> simp[]
     ) >>
   Cases_on `s = "Update"` >> gvs[]
   >- (
-    IF_CASES_TAC >> gvs[] >> rw[twith_atoms_def] >>
+    IF_CASES_TAC >> gvs[] >> rw[with_atoms_def] >>
     ntac 6 (TOP_CASE_TAC >> gvs[]) >>
     first_x_assum irule >> simp[] >> qexists_tac `[Loc n; Int i]` >> simp[]
     )
@@ -257,7 +256,7 @@ Theorem next_next:
   next n e k st ≠ Div ∧ next m e k st ≠ Div ⇒
   next n e k st = next m e k st
 Proof
-  metis_tac [arithmeticTheory.LESS_EQ_CASES, tnext_less_eq]
+  metis_tac [arithmeticTheory.LESS_EQ_CASES, next_less_eq]
 QED
 
 
